logic-py/Transform.py
@@ -19,13 +19,21 @@ class default__:
 
     @staticmethod
     def ReverseRow(row):
-        return _dafny.SeqWithoutIsStrInference([(row)[3], (row)[2], (row)[1], (row)[0]])
+        return _dafny.SeqWithoutIsStrInference([(row)[((Setups.default__.N) - (1)) - (d_0_j_)] for d_0_j_ in range(Setups.default__.N)])
 
     @staticmethod
     def Reverse(grid):
-        return _dafny.SeqWithoutIsStrInference([default__.ReverseRow((grid)[0]), default__.ReverseRow((grid)[1]), default__.ReverseRow((grid)[2]), default__.ReverseRow((grid)[3])])
+        return _dafny.SeqWithoutIsStrInference([default__.ReverseRow((grid)[d_0_i_]) for d_0_i_ in range(Setups.default__.N)])
+
+    @staticmethod
+    def twotilesadjacent(i, j, grid):
+        return Setups.default__.VerticalPair(i, j, grid)
+
+    @staticmethod
+    def twotilesadjacentrow(i, j, grid):
+        return Setups.default__.HorizontalPair(i, j, grid)
 
     @staticmethod
     def Transpose(grid):
-        return _dafny.SeqWithoutIsStrInference([_dafny.SeqWithoutIsStrInference([((grid)[0])[0], ((grid)[1])[0], ((grid)[2])[0], ((grid)[3])[0]]), _dafny.SeqWithoutIsStrInference([((grid)[0])[1], ((grid)[1])[1], ((grid)[2])[1], ((grid)[3])[1]]), _dafny.SeqWithoutIsStrInference([((grid)[0])[2], ((grid)[1])[2], ((grid)[2])[2], ((grid)[3])[2]]), _dafny.SeqWithoutIsStrInference([((grid)[0])[3], ((grid)[1])[3], ((grid)[2])[3], ((grid)[3])[3]])])
+        return _dafny.SeqWithoutIsStrInference([_dafny.SeqWithoutIsStrInference([((grid)[d_0_j_])[d_1_i_] for d_0_j_ in range(Setups.default__.N)]) for d_1_i_ in range(Setups.default__.N)])
 
